Dirty commit.

reflex/coq/bench-quark/PolicyNonInterference.v
@@ -2,23 +2,14 @@ Require Import Kernel NIExists Reflex ReflexBase ReflexFin ReflexHVec.
 
 Import SystemFeatures.
 
-Definition clblr d (c : comp COMPT COMPS) :=
-  match c
-  with
-  | Build_comp Tab _ cfg =>
-    let cfgd := comp_conf_desc COMPT COMPS Tab in
-    if str_eq (@shvec_ith _ _ (projT1 cfgd) (projT2 cfgd)
-                               cfg None) d
-    then true
-    else false
-  | Build_comp CProc _ cfg =>
-    let cfgd := comp_conf_desc COMPT COMPS Tab in
-    if str_eq (@shvec_ith _ _ (projT1 cfgd) (projT2 cfgd)
-                               cfg None) d
-    then true
-    else false
-  | Build_comp UserInput _ _ => true
-  | _ => false
+Definition clblr (d:str) (ct:COMPT) :
+  option (shvec sdenote_desc_conc_pat
+    (projT2 (comp_conf_desc COMPT COMPS ct))) :=
+  match ct with
+  | Tab => Some (Some d, tt)
+  | CProc => Some (Some d, tt)
+  | UserInput => Some tt
+  | _ => None
   end.
 
 Definition vlblr (f : fin (projT1 KSTD)) := true.
@@ -27,8 +18,71 @@ Local Opaque str_of_string.
 
 Import Language Spec.
 
+  Ltac destruct_msg' :=
+  match goal with
+  | [ m : msg _ |- _ ]
+      => let tag := fresh "tag" in
+         let pay := fresh "pay" in
+         destruct m as [tag pay]; destruct_fin tag
+  end.
+
+
+Ltac destruct_comp' :=
+  match goal with
+  | [ c : Reflex.comp _ _ |- _ ]
+      => let ct := fresh "ct" in
+         let cfd := fresh "cfd" in
+         let cfg := fresh "cfg" in
+         destruct c as [ct cfd cfg];
+         destruct ct
+  end.
+
+Require Import PruneFacts.
+
 Theorem ni : forall d, NI PAYD COMPT COMPTDEC COMPS
   IENVD KSTD INIT HANDLERS (clblr d) vlblr.
 Proof.
+  intros. apply ni_suf_all.
+
+Local Opaque cmd_ok_low.
+Ltac low_solve :=
+  repeat first
+        [ apply nop_low |
+          apply seq_low |
+          apply ite_low |
+          apply complkup_low |
+          apply call_low |
+          apply send_low_ccomp |
+          apply stupd_low |
+          solve [auto] ].
+    Time unfold low_ok''; intros; destruct_msg'; destruct_comp'; simpl;
+      try discriminate; low_solve. admit. admit. admit. admit.
+
+Ltac high_solve :=
+  repeat first
+    [ apply nop_high_all |
+      apply seq_high_all |
+      apply ite_high_all |
+      apply complkup_high_all |
+      apply call_high_all |
+      apply spawn_high_all |
+      apply send_high_all |
+      apply stupd_high_all |
+      solve [auto] ].
+
+Local Opaque all_cmd_ok_high.
+
+    Time unfold high_ok_all; intros; destruct_msg'; destruct_comp'; simpl;
+      try discriminate; high_solve. simpl. unfold hdlr_tab_dom. unfold is_high_comp_pat. simpl.
+      repeat first
+        [ apply nop_high_all |
+          apply seq_low |
+          apply ite_low |
+          apply complkup_low |
+          apply call_low |
+          apply send_low_ccomp |
+          apply stupd_low |
+          solve [auto] ].
+
   Time ni.
 Qed.
